[temporal_deep] abstract LTL3 and PTLTL monitors; more theorems about LTL_TO_GEN_BUECHI translations

examples/temporal_deep/src/examples/runtime_verificationScript.sml
@@ -7,10 +7,14 @@
 open HolKernel Parse boolLib bossLib;
 
 (* standard libraries & utilities *)
-open optionTheory listTheory rich_listTheory arithmeticTheory hurdUtils;
+open pairTheory optionTheory listTheory pred_setTheory rich_listTheory
+     arithmeticTheory hurdUtils combinTheory;
 
 (* local theories *)
-open prop_logicTheory full_ltlTheory translationsLib ltl_to_automaton_formulaTheory;
+open prop_logicTheory xprop_logicTheory full_ltlTheory translationsLib
+     symbolic_kripke_structureTheory symbolic_semi_automatonTheory
+     automaton_formulaTheory ltl_to_automaton_formulaTheory
+     omega_automaton_translationsTheory temporal_deep_mixedTheory;
 
 (* Tuerk's translations between different LTL syntax (unused)
 open ltl_translationsTheory;
@@ -32,14 +36,13 @@ val _ = overload_on ("LTL3_T", ``SOME T``);     (* conclusive true *)
 val _ = overload_on ("LTL3_F", ``SOME F``);     (* conclusive false *)
 val _ = overload_on ("LTL3_U", ``NONE :LTL3``); (* inconclusive/unknown *)
 
-(* ABRV-LTL (unused)
+(* ABRV-LTL *)
 val _ = type_abbrev_pp ("ABRV_LTL", ``:LTL3 option``);
 
 val _ = overload_on ("true",    ``SOME LTL3_T``);
 val _ = overload_on ("false",   ``SOME LTL3_F``);
 val _ = overload_on ("unknown", ``SOME LTL3_U``);
-val _ = overload_on ("out_of_model", ``NONE :ABRV_LTL``);
- *)
+val _ = overload_on ("error",   ``NONE :ABRV_LTL``);
 
 Theorem THE_LTL3 :
    (THE LTL3_T = T) /\ (THE LTL3_F = F)
@@ -231,15 +234,15 @@ Proof
       METIS_TAC [] )
 QED
 
-Definition IS_CONCL_def :
-    IS_CONCL x = ((x = LTL3_T) \/ (x = LTL3_F))
+Definition LTL3_IS_CONCL_def :
+    LTL3_IS_CONCL x = ((x = LTL3_T) \/ (x = LTL3_F))
 End
 
 (* LTL3 semantic of ptLTL is always conclusive *)
 Theorem PTLTL_SEM_LTL3_CONCL :
-    !f u i. i < LENGTH u /\ IS_PAST_LTL f ==> IS_CONCL (LTL3_SEM_TIME i u f)
+    !f u i. i < LENGTH u /\ IS_PAST_LTL f ==> LTL3_IS_CONCL (LTL3_SEM_TIME i u f)
 Proof
-    RW_TAC std_ss [IS_CONCL_def, LTL3_SEM_TIME_def]
+    RW_TAC std_ss [LTL3_IS_CONCL_def, LTL3_SEM_TIME_def]
  >> METIS_TAC [PTLTL_SEM_THM]
 QED
 
@@ -249,9 +252,9 @@ Theorem PTLTL_SEM_LTL3_AND :
                 THE (LTL3_SEM_TIME i u f1) /\ THE (LTL3_SEM_TIME i u f2))
 Proof
     rpt STRIP_TAC
- >> `IS_CONCL (LTL3_SEM_TIME i u f1) /\
-     IS_CONCL (LTL3_SEM_TIME i u f2)` by PROVE_TAC [PTLTL_SEM_LTL3_CONCL]
- >> fs [IS_CONCL_def, LTL3_SEM_TIME_def, LTL_SEM_TIME_def]
+ >> `LTL3_IS_CONCL (LTL3_SEM_TIME i u f1) /\
+     LTL3_IS_CONCL (LTL3_SEM_TIME i u f2)` by PROVE_TAC [PTLTL_SEM_LTL3_CONCL]
+ >> fs [LTL3_IS_CONCL_def, LTL3_SEM_TIME_def, LTL_SEM_TIME_def]
  >| [ (* goal 1 (of 4) *)
       `!w. LTL_SEM_TIME i (u ++ w) f1` by METIS_TAC [LTL3_distinct] \\
       `!w. LTL_SEM_TIME i (u ++ w) f2` by METIS_TAC [LTL3_distinct],
@@ -309,13 +312,13 @@ Proof
        (MP_TAC o (Q.SPEC `BUTLASTN 1 u`)) \\
      RW_TAC arith_ss [LENGTH_BUTLASTN] \\
      POP_ASSUM K_TAC \\ (* IH1 leftover removed *)
-     Know `IS_CONCL (LTL3_SEM_TIME (LENGTH u − 1) u (LTL_PREV f))`
+     Know `LTL3_IS_CONCL (LTL3_SEM_TIME (LENGTH u − 1) u (LTL_PREV f))`
      >- (MATCH_MP_TAC PTLTL_SEM_LTL3_CONCL >> rw [IS_PAST_LTL_def]) \\
-     Know `IS_CONCL (LTL3_SEM_TIME (LENGTH u − 2) (BUTLASTN 1 u) f)`
+     Know `LTL3_IS_CONCL (LTL3_SEM_TIME (LENGTH u − 2) (BUTLASTN 1 u) f)`
      >- (MATCH_MP_TAC PTLTL_SEM_LTL3_CONCL >> rw [LENGTH_BUTLASTN]) \\
      (* 4 combinations of LTL3_T and LTL3_F *)
      RW_TAC (bool_ss ++ ARITH_ss)
-            [IS_CONCL_def, LTL3_SEM_TIME_def, LTL_SEM_TIME_def, PRE_SUB1] >|
+            [LTL3_IS_CONCL_def, LTL3_SEM_TIME_def, LTL_SEM_TIME_def, PRE_SUB1] >|
      (* 2 impossible cases left *)
      [ (* goal 4.1 (of 2) *)
        Q.PAT_X_ASSUM `!w. LTL_SEM_TIME (LENGTH u - 2) _ f`
@@ -329,12 +332,12 @@ Proof
        rw [APPEND_BUTLASTN_LASTN] ])
  (* goal 5 (of 5): LTL_SINCE *)
  >> RW_TAC std_ss [PTLTL_SEM_ALT_def]
- >> Know `IS_CONCL (LTL3_SEM_TIME (LENGTH u - 1) u (LTL_SINCE (f,f')))`
+ >> Know `LTL3_IS_CONCL (LTL3_SEM_TIME (LENGTH u - 1) u (LTL_SINCE (f,f')))`
  >- (MATCH_MP_TAC PTLTL_SEM_LTL3_CONCL \\
      CONJ_TAC >- RW_TAC arith_ss [] \\
      PROVE_TAC [IS_PAST_LTL_def])
  >> RW_TAC std_ss (* or: (bool_ss ++ ARITH_ss) to see things more clearly *)
-          [LTL3_SEM_TIME_def, LTL_SEM_TIME_def, IS_CONCL_def]
+          [LTL3_SEM_TIME_def, LTL_SEM_TIME_def, LTL3_IS_CONCL_def]
  >| [ (* goal 5.1 (of 2) *)
       POP_ASSUM (STRIP_ASSUME_TAC o (Q.SPEC `\i. {}`)) \\
       Q.EXISTS_TAC `LENGTH u - 1 - k` (* `j + 1` in paper notation *) \\
@@ -342,18 +345,18 @@ Proof
       CONJ_TAC (* PTLTL_SEM_ALT (BUTLASTN (LENGTH u - 1 - k) u) f' *)
       >- (`(k = LENGTH u - 1) \/ k < LENGTH u - 1` by RW_TAC arith_ss []
           >- (fs [BUTLASTN] \\
-              Know `IS_CONCL (LTL3_SEM_TIME (LENGTH u - 1) u f')`
+              Know `LTL3_IS_CONCL (LTL3_SEM_TIME (LENGTH u - 1) u f')`
               >- (MATCH_MP_TAC PTLTL_SEM_LTL3_CONCL >> rw []) \\
-              rw [LTL3_SEM_TIME_def, IS_CONCL_def] >> fs []) \\
+              rw [LTL3_SEM_TIME_def, LTL3_IS_CONCL_def] >> fs []) \\
           (* now `k < LENGTH u - 1` *)
           Q.PAT_X_ASSUM `!y. LENGTH y < LENGTH u ==> _`
              (MP_TAC o (Q.SPEC `BUTLASTN (LENGTH u - 1 - k) u`)) \\
           RW_TAC arith_ss [LENGTH_BUTLASTN] \\
           POP_ASSUM (MP_TAC o (Q.SPEC `f'`)) >> RW_TAC std_ss [] \\
           POP_ASSUM K_TAC (* cleanup *) \\
-          Know `IS_CONCL (LTL3_SEM_TIME k (BUTLASTN (LENGTH u - (k + 1)) u) f')`
+          Know `LTL3_IS_CONCL (LTL3_SEM_TIME k (BUTLASTN (LENGTH u - (k + 1)) u) f')`
           >- (MATCH_MP_TAC PTLTL_SEM_LTL3_CONCL >> rw [LENGTH_BUTLASTN]) \\
-          rw [LTL3_SEM_TIME_def, IS_CONCL_def] \\
+          rw [LTL3_SEM_TIME_def, LTL3_IS_CONCL_def] \\
           POP_ASSUM (MP_TAC o (ONCE_REWRITE_RULE [GSYM concat_assoc]) o
                      (Q.SPEC `(LASTN (LENGTH u - (k + 1)) u) ++ (\i. {})`)) \\
           rw [APPEND_BUTLASTN_LASTN]) \\
@@ -361,9 +364,9 @@ Proof
       rpt STRIP_TAC \\
      `(j = 0) \/ 0 < j` by RW_TAC arith_ss [] (* `i = n \/ i < n` in paper *)
       >- (rw [BUTLASTN] \\
-          Know `IS_CONCL (LTL3_SEM_TIME (LENGTH u - 1) u f)`
+          Know `LTL3_IS_CONCL (LTL3_SEM_TIME (LENGTH u - 1) u f)`
           >- (MATCH_MP_TAC PTLTL_SEM_LTL3_CONCL >> rw []) \\
-          rw [LTL3_SEM_TIME_def, IS_CONCL_def] \\
+          rw [LTL3_SEM_TIME_def, LTL3_IS_CONCL_def] \\
           Q.PAT_X_ASSUM `!j. k < j /\ j <= LENGTH u - 1 ==> _`
              (MP_TAC o (Q.SPEC `LENGTH (u :'a set list) - 1`)) \\
           RW_TAC arith_ss []) \\
@@ -371,9 +374,9 @@ Proof
       Q.PAT_X_ASSUM `!y. LENGTH y < LENGTH u ==> _`
          (MP_TAC o (Q.SPEC `BUTLASTN j u`)) >> rw [LENGTH_BUTLASTN] \\
       POP_ASSUM K_TAC (* cleanup *) \\
-      Know `IS_CONCL (LTL3_SEM_TIME (LENGTH u − (j + 1)) (BUTLASTN j u) f)`
+      Know `LTL3_IS_CONCL (LTL3_SEM_TIME (LENGTH u − (j + 1)) (BUTLASTN j u) f)`
       >- (MATCH_MP_TAC PTLTL_SEM_LTL3_CONCL >> rw [LENGTH_BUTLASTN]) \\
-      rw [LTL3_SEM_TIME_def, IS_CONCL_def] \\
+      rw [LTL3_SEM_TIME_def, LTL3_IS_CONCL_def] \\
       Q.PAT_X_ASSUM `!j. k < j /\ j <= LENGTH u - 1 ==> _`
          (MP_TAC o (Q.SPEC `LENGTH (u :'a set list) - (j + 1)`)) \\
       RW_TAC arith_ss [] \\
@@ -386,10 +389,10 @@ Proof
          (ASSUME_TAC o (Q.SPEC `\i. {}`)) \\
      `(k = 0) \/ 0 < k` by RW_TAC arith_ss []
       >- (fs [BUTLASTN] \\
-          Know `IS_CONCL (LTL3_SEM_TIME (LENGTH u − 1) u f')`
+          Know `LTL3_IS_CONCL (LTL3_SEM_TIME (LENGTH u − 1) u f')`
           >- (MATCH_MP_TAC PTLTL_SEM_LTL3_CONCL >> rw []) \\
           Q.PAT_X_ASSUM `THE (LTL3_SEM_TIME (LENGTH u − 1) u f')` MP_TAC \\
-          rw [LTL3_SEM_TIME_def, IS_CONCL_def] \\
+          rw [LTL3_SEM_TIME_def, LTL3_IS_CONCL_def] \\
           Q.PAT_X_ASSUM `!k. ~(k <= LENGTH u - 1) \/ _`
              (MP_TAC o (Q.SPEC `LENGTH (u :'a set list) - 1`)) \\
           RW_TAC arith_ss []) \\
@@ -398,9 +401,9 @@ Proof
       >- (FIRST_X_ASSUM irule (* IH *) >> rw [LENGTH_BUTLASTN]) \\
       rw [LENGTH_BUTLASTN] \\
       POP_ASSUM MP_TAC \\
-      Know `IS_CONCL (LTL3_SEM_TIME (LENGTH u − (k + 1)) (BUTLASTN k u) f')`
+      Know `LTL3_IS_CONCL (LTL3_SEM_TIME (LENGTH u − (k + 1)) (BUTLASTN k u) f')`
       >- (MATCH_MP_TAC PTLTL_SEM_LTL3_CONCL >> rw [LENGTH_BUTLASTN]) \\
-      rw [LTL3_SEM_TIME_def, IS_CONCL_def] \\
+      rw [LTL3_SEM_TIME_def, LTL3_IS_CONCL_def] \\
       POP_ASSUM (MP_TAC o (ONCE_REWRITE_RULE [GSYM concat_assoc]) o
                  (Q.SPEC `(LASTN k u) ++ (\i. {})`)) \\
       rw [APPEND_BUTLASTN_LASTN] \\
@@ -409,21 +412,183 @@ Proof
       RW_TAC arith_ss [] \\
      `(j = LENGTH u - 1) \/ (j < LENGTH u - 1)` by RW_TAC arith_ss []
       >- (Q.EXISTS_TAC `0` >> rw [BUTLASTN] \\
-          Know `IS_CONCL (LTL3_SEM_TIME (LENGTH u − 1) u f)`
+          Know `LTL3_IS_CONCL (LTL3_SEM_TIME (LENGTH u − 1) u f)`
           >- (MATCH_MP_TAC PTLTL_SEM_LTL3_CONCL >> rw []) \\
-          rw [LTL3_SEM_TIME_def, IS_CONCL_def] >> fs []) \\
+          rw [LTL3_SEM_TIME_def, LTL3_IS_CONCL_def] >> fs []) \\
       (* final part *)
       Q.EXISTS_TAC `LENGTH u - (j + 1)` >> rw [] \\
       Q.PAT_X_ASSUM `!y. LENGTH y < LENGTH u ==> _`
          (MP_TAC o (Q.SPEC `BUTLASTN (LENGTH u - (j + 1)) u`)) \\
       rw [LENGTH_BUTLASTN] \\
       POP_ASSUM K_TAC (* cleanup *) \\
-      Know `IS_CONCL (LTL3_SEM_TIME j (BUTLASTN (LENGTH u − (j + 1)) u) f)`
+      Know `LTL3_IS_CONCL (LTL3_SEM_TIME j (BUTLASTN (LENGTH u − (j + 1)) u) f)`
       >- (MATCH_MP_TAC PTLTL_SEM_LTL3_CONCL >> rw [LENGTH_BUTLASTN]) \\
-      rw [LTL3_SEM_TIME_def, IS_CONCL_def] \\
+      rw [LTL3_SEM_TIME_def, LTL3_IS_CONCL_def] \\
       POP_ASSUM (MP_TAC o (ONCE_REWRITE_RULE [GSYM concat_assoc]) o
                   (Q.SPEC `(LASTN (LENGTH u - (j + 1)) u) ++ (\i. {})`)) \\
       rw [APPEND_BUTLASTN_LASTN] ]
+QED
+
+(* -------------------------------------------------------------------------- *)
+(*   LTL3 and PTLTL monitors (abstract version)                               *)
+(* -------------------------------------------------------------------------- *)
+
+val _ = set_fixity "extends" (Infix(NONASSOC, 450));
+
+Definition extends_def : (* no partial observability *)
+    (i extends u) = ?c. i = concat u c
+End
+
+Definition LTL3_output_def :
+   (LTL3_output T T = LTL3_U) /\
+   (LTL3_output T F = LTL3_T) /\
+   (LTL3_output F T = LTL3_F)
+End
+
+Definition ABRV_output_def : (* not used, for comparison only *)
+   (ABRV_output T T = unknown) /\
+   (ABRV_output T F = true) /\
+   (ABRV_output F T = false) /\
+   (ABRV_output F F = error)
+End
+
+(* "belief run" after taking a finite trace u *)
+Definition LTL3_belief_run_def :
+    LTL3_belief_run l u = {i | i extends u /\ LTL_SEM i l}
+End
+
+(* LTL3 monitor (abstract version) *)
+Definition LTL3_monitor_def :
+    LTL3_monitor l u = LTL3_output (LTL3_belief_run l           u <> EMPTY)
+                                   (LTL3_belief_run (LTL_NOT l) u <> EMPTY)
+End
+
+(* correctness of LTL3 monitor, an abstract version *)
+Theorem LTL3_monitor_thm :
+    !l u. LTL3_monitor l u = LTL3_SEM u l
+Proof
+    RW_TAC std_ss [LTL3_monitor_def, LTL3_SEM_def]
+ >> Cases_on `LTL3_belief_run          l  u = {}`
+ >> Cases_on `LTL3_belief_run (LTL_NOT l) u = {}`
+ >> fs [LTL3_output_def] (* 4 subgoals *)
+ >| [ (* goal 1 (of 4) *)
+      fs [LTL3_belief_run_def, EXTENSION, NOT_IN_EMPTY, GSPECIFICATION,
+          LTL_SEM_def, LTL_SEM_TIME_def] \\
+      Q.ABBREV_TAC `i = u ++ (\n. {})` \\
+     `i extends u` by PROVE_TAC [extends_def] \\
+      METIS_TAC [],
+      (* goal 2 (of 4) *)
+      RW_TAC std_ss [Once EQ_SYM_EQ, LTL3_SEM_def, LTL3_SEM_TIME_F] \\
+      Q.PAT_X_ASSUM `LTL3_belief_run (LTL_NOT l) u <> {}` K_TAC \\
+      fs [LTL3_belief_run_def, EXTENSION, NOT_IN_EMPTY, GSPECIFICATION,
+          LTL_SEM_def, LTL_SEM_TIME_def] \\
+      POP_ASSUM (MP_TAC o (Q.SPEC `u ++ v`)) \\
+     `u ++ v extends u` by PROVE_TAC [extends_def] \\
+      METIS_TAC [],
+      (* goal 3 (of 4) *)
+      RW_TAC std_ss [Once EQ_SYM_EQ, LTL3_SEM_def, LTL3_SEM_TIME_T] \\
+      Q.PAT_X_ASSUM `LTL3_belief_run l u <> {}` K_TAC \\
+      fs [LTL3_belief_run_def, EXTENSION, NOT_IN_EMPTY, GSPECIFICATION,
+          LTL_SEM_def, LTL_SEM_TIME_def] \\
+      POP_ASSUM (MP_TAC o (Q.SPEC `u ++ v`)) \\
+     `u ++ v extends u` by PROVE_TAC [extends_def] \\
+      METIS_TAC [],
+      (* goal 4 (of 4) *)
+      RW_TAC std_ss [Once EQ_SYM_EQ, LTL3_SEM_def, LTL3_SEM_TIME_def] >|
+      [ (* goal 4.1 (of 2) *)
+        Q.PAT_X_ASSUM `LTL3_belief_run l u <> {}` K_TAC \\
+        fs [LTL3_belief_run_def, EXTENSION, NOT_IN_EMPTY, GSPECIFICATION,
+            LTL_SEM_def, LTL_SEM_TIME_def, extends_def] \\
+        POP_ASSUM (STRIP_ASSUME_TAC o (Q.SPEC `c`)) \\
+        METIS_TAC [],
+        (* goal 4.2 (of 2) *)
+        Q.PAT_X_ASSUM `~!w. P` K_TAC \\
+        Q.PAT_X_ASSUM `LTL3_belief_run (LTL_NOT l) u <> {}` K_TAC \\
+        fs [LTL3_belief_run_def, EXTENSION, NOT_IN_EMPTY, GSPECIFICATION,
+            LTL_SEM_def, LTL_SEM_TIME_def, extends_def] \\
+        POP_ASSUM (STRIP_ASSUME_TAC o (Q.SPEC `c`)) \\
+        METIS_TAC [] ] ]
+QED
+
+Definition GEN_LTL3_belief_run_def :
+    GEN_LTL3_belief_run l u t = {i | i extends u /\ LTL_SEM_TIME t i l}
+End
+
+(* alternative definition *)
+Theorem LTL3_belief_run_alt :
+    !l u. LTL3_belief_run l u = GEN_LTL3_belief_run l u 0
+Proof
+    RW_TAC std_ss [GEN_LTL3_belief_run_def, LTL3_belief_run_def, LTL_SEM_def]
+QED
+
+(* LTL3 monitor (abstract version) *)
+Definition GEN_LTL3_monitor_def :
+    GEN_LTL3_monitor l u t =
+        LTL3_output (GEN_LTL3_belief_run l           u t <> EMPTY)
+                    (GEN_LTL3_belief_run (LTL_NOT l) u t <> EMPTY)
+End
+
+(* alternative definition *)
+Theorem LTL3_monitor_alt :
+    !l u. LTL3_monitor l u = GEN_LTL3_monitor l u 0
+Proof
+    RW_TAC std_ss [GEN_LTL3_monitor_def, GSYM LTL3_belief_run_alt,
+                   LTL3_monitor_def]
+QED
+
+(* correctness of LTL3 monitor, an abstract version *)
+Theorem GEN_LTL3_monitor_thm :
+    !l u t. GEN_LTL3_monitor l u t = LTL3_SEM_TIME t u l
+Proof
+    RW_TAC std_ss [GEN_LTL3_monitor_def]
+ >> Cases_on `GEN_LTL3_belief_run          l  u t = {}`
+ >> Cases_on `GEN_LTL3_belief_run (LTL_NOT l) u t = {}`
+ >> fs [LTL3_output_def] (* 4 subgoals *)
+ >| [ (* goal 1 (of 4) *)
+      fs [GEN_LTL3_belief_run_def, EXTENSION, NOT_IN_EMPTY, GSPECIFICATION,
+          LTL_SEM_TIME_def] \\
+      Q.ABBREV_TAC `i = u ++ (\n. {})` \\
+     `i extends u` by PROVE_TAC [extends_def] \\
+      METIS_TAC [],
+      (* goal 2 (of 4) *)
+      RW_TAC std_ss [Once EQ_SYM_EQ, LTL3_SEM_TIME_F] \\
+      Q.PAT_X_ASSUM `GEN_LTL3_belief_run (LTL_NOT l) u t <> {}` K_TAC \\
+      fs [GEN_LTL3_belief_run_def, EXTENSION, NOT_IN_EMPTY, GSPECIFICATION,
+          LTL_SEM_TIME_def] \\
+      POP_ASSUM (MP_TAC o (Q.SPEC `u ++ v`)) \\
+     `u ++ v extends u` by PROVE_TAC [extends_def] \\
+      METIS_TAC [],
+      (* goal 3 (of 4) *)
+      RW_TAC std_ss [Once EQ_SYM_EQ, LTL3_SEM_TIME_T] \\
+      Q.PAT_X_ASSUM `GEN_LTL3_belief_run l u t <> {}` K_TAC \\
+      fs [GEN_LTL3_belief_run_def, EXTENSION, NOT_IN_EMPTY, GSPECIFICATION,
+          LTL_SEM_TIME_def] \\
+      POP_ASSUM (MP_TAC o (Q.SPEC `u ++ v`)) \\
+     `u ++ v extends u` by PROVE_TAC [extends_def] \\
+      METIS_TAC [],
+      (* goal 4 (of 4) *)
+      RW_TAC std_ss [Once EQ_SYM_EQ, LTL3_SEM_TIME_def] >|
+      [ (* goal 4.1 (of 2) *)
+        Q.PAT_X_ASSUM `GEN_LTL3_belief_run l u t <> {}` K_TAC \\
+        fs [GEN_LTL3_belief_run_def, EXTENSION, NOT_IN_EMPTY, GSPECIFICATION,
+            LTL_SEM_TIME_def, extends_def] \\
+        POP_ASSUM (STRIP_ASSUME_TAC o (Q.SPEC `c`)) \\
+        METIS_TAC [],
+        (* goal 4.2 (of 2) *)
+        Q.PAT_X_ASSUM `~!w. P` K_TAC \\
+        Q.PAT_X_ASSUM `GEN_LTL3_belief_run (LTL_NOT l) u t <> {}` K_TAC \\
+        fs [GEN_LTL3_belief_run_def, EXTENSION, NOT_IN_EMPTY, GSPECIFICATION,
+            LTL_SEM_TIME_def, extends_def] \\
+        POP_ASSUM (STRIP_ASSUME_TAC o (Q.SPEC `c`)) \\
+        METIS_TAC [] ] ]
+QED
+
+(* PTLTL monitor *)
+Theorem PTLTL_monitor_thm :
+    !f u. IS_PAST_LTL f /\ 0 < LENGTH u ==>
+         (PTLTL_SEM_ALT u f = THE (GEN_LTL3_monitor f u (LENGTH u - 1)))
+Proof
+    RW_TAC std_ss [PTLTL_SEM_ALT_LTL3, GEN_LTL3_monitor_thm]
 QED
 
 val _ = export_theory ();
